wip

clightlight/SimSTS3.v
@@ -676,12 +676,10 @@ Section SIM.
 
   Variable L0: STS.semantics.
   Variable L1: Smallstep.semantics.
-  Let idx := Ord.t.
-  Let ord := Ord.lt.
 
   Local Open Scope smallstep_scope.
 
-  Variant _sim sim (i0: idx) (st_src0: L0.(STS.state)) (st_tgt0: L1.(Smallstep.state)): Prop :=
+  Variant _sim sim (f_src f_tgt: bool) (st_src0: L0.(STS.state)) (st_tgt0: L1.(Smallstep.state)): Prop :=
   | sim_fin
       retv
       (RANGE: (0 <= retv <= Int.max_unsigned)%Z)
@@ -690,7 +688,7 @@ Section SIM.
       (SRT: _.(Smallstep.final_state) st_tgt0 (Int.repr retv))
       (* (DTM: True) (*** TODO: copy-paste sd_final_determ in Smallstep.v ***) *)
     :
-      _sim sim i0 st_src0 st_tgt0
+      _sim sim f_src f_tgt st_src0 st_tgt0
 
   | sim_vis
       (SRT: _.(state_sort) st_src0 = vis)
@@ -700,18 +698,18 @@ Section SIM.
         ,
           exists st_src1 ev_src (STEP: _.(step) st_src0 (Some ev_src) st_src1),
             (<<MATCH: Forall2 match_event ev_tgt [ev_src]>>) /\
-            (<<SIM: exists i1, sim i1 st_src1 st_tgt1>>))
+            (<<SIM: sim true true st_src1 st_tgt1>>))
     :
-      _sim sim i0 st_src0 st_tgt0
+      _sim sim f_src f_tgt st_src0 st_tgt0
 
   | sim_demonic_src
       (SRT: _.(state_sort) st_src0 = demonic)
       (SIM: exists st_src1
           (STEP: _.(step) st_src0 None st_src1)
         ,
-          exists i1, <<ORD: ord i1 i0>> /\ <<SIM: sim i1 st_src1 st_tgt0>>)
+          <<SIM: sim true f_tgt st_src1 st_tgt0>>)
     :
-      _sim sim i0 st_src0 st_tgt0
+      _sim sim f_src f_tgt st_src0 st_tgt0
   | sim_demonic_tgt_dtm
       (*** WRONG DEF, Note: UB in tgt ***)
       (* (SIM: forall st_tgt1 *)
@@ -721,7 +719,7 @@ Section SIM.
       (SIM: exists st_tgt1
           (STEP: Step L1 st_tgt0 E0 st_tgt1)
         ,
-          exists i1, <<ORD: ord i1 i0>> /\ <<SIM: sim i1 st_src0 st_tgt1>>)
+          <<SIM: sim f_src true st_src0 st_tgt1>>)
       (*** equivalent def ***)
       (* st_tgt1 *)
       (* (STEP: Step L1 st_tgt0 E0 st_tgt1) *)
@@ -729,17 +727,16 @@ Section SIM.
       (* (ORD: ord i1 i0) *)
       (* (SIM: sim i1 st_src0 st_tgt1) *)
     :
-      _sim sim i0 st_src0 st_tgt0
+      _sim sim f_src f_tgt st_src0 st_tgt0
   | sim_angelic_src
       (SRT: _.(state_sort) st_src0 = angelic)
       (DTM: forall st1 st2, (<<DTM1: _.(step) st_src0 None st1>>) -> (<<DTM2: _.(step) st_src0 None st2>>) -> st1 = st2)
       (SIM: forall st_src1
           (STEP: _.(step) st_src0 None st_src1)
         ,
-          exists i1, <<ORD: ord i1 i0>> /\ <<SIM: sim i1 st_src1 st_tgt0>>)
+          <<SIM: sim true f_tgt st_src1 st_tgt0>>)
     :
-      _sim sim i0 st_src0 st_tgt0
-
+      _sim sim f_src f_tgt st_src0 st_tgt0
 
   | sim_demonic_both
       (SRT: _.(state_sort) st_src0 = demonic)
@@ -747,14 +744,21 @@ Section SIM.
           (STEP: Step L1 st_tgt0 E0 st_tgt1)
         ,
           exists st_src1 (STEP: _.(step) st_src0 None st_src1),
-            <<SIM: exists i1, sim i1 st_src1 st_tgt1>>)
+            <<SIM: sim true true st_src1 st_tgt1>>)
     :
-      _sim sim i0 st_src0 st_tgt0
+      _sim sim f_src f_tgt st_src0 st_tgt0
+  
+  | sim_progress 
+      (SIM: sim false false st_src0 st_tgt0)
+      (SRC: f_src = true)
+      (TGT: f_tgt = true)
+    :
+      _sim sim f_src f_tgt st_src0 st_tgt0
   .
 
-  Definition sim: _ -> _ -> _ -> Prop := paco3 _sim bot3.
+  Definition sim: _ -> _ -> _ -> _ -> Prop := paco4 _sim bot4.
 
-  Lemma sim_mon: monotone3 _sim.
+  Lemma sim_mon: monotone4 _sim.
   Proof.
     ii. inv IN.
 
@@ -762,8 +766,9 @@ Section SIM.
     - econs 2; et. i. exploit SIM; et. i; des. esplits; et.
     - econs 3; et. des. esplits; et.
     - econs 4; et. des. esplits; et.
-    - econs 5; et. i. exploit SIM; et. i; des. esplits; et.
+    - econs 5; et. i. exploit SIM; et.
     - econs 6; et. des. esplits; et.
+    - econs 7; et.
   Qed.
 
   Hint Constructors _sim.
@@ -771,7 +776,7 @@ Section SIM.
   Hint Resolve sim_mon: paco.
 
 
-  Variant ordC (r: idx -> L0.(STS.state) -> L1.(Smallstep.state) -> Prop):
+  (* Variant ordC (r: idx -> L0.(STS.state) -> L1.(Smallstep.state) -> Prop):
     idx -> L0.(STS.state) -> L1.(Smallstep.state) -> Prop :=
   | ordC_intro
       o0 o1 st_src st_tgt
@@ -809,18 +814,18 @@ Section SIM.
     intros. gclo. econs.
     { eapply ordC_compatible. }
     eapply ordC_mon; [|et]. i. gbase. auto.
-  Qed.
+  Qed. *)
 
   Record simulation: Prop := mk_simulation {
     sim_init: forall st_tgt0 (INITT: L1.(Smallstep.initial_state) st_tgt0),
-        exists i0, (<<SIM: sim i0 L0.(initial_state) st_tgt0>>);
+        (<<SIM: sim false false L0.(initial_state) st_tgt0>>);
     (* sim_init: exists i0 st_tgt0, (<<SIM: sim i0 L0.(initial_state) st_tgt0>>) /\ *)
     (*                              (<<INITT: L1.(Smallstep.initial_state) st_tgt0>>); *)
     (* sim_dtm: True; *)
   }
   .
 
-  Hypothesis WF: well_founded ord.
+  (* Hypothesis WF: well_founded ord. *)
   Hypothesis WFSEM: wf_semantics L1.
 
   Ltac pc H := rr in H; desH H; ss.
@@ -953,7 +958,11 @@ Section SIM.
 
   (* Hypothesis WFSRC: wf L0. *)
 
-  Lemma simulation_star
+  (* 
+  TODO : update adequacy 
+   *)
+
+  (* Lemma simulation_star
         i0 st_src0 tr_tgt st_tgt1 st_tgt0
         (* (MATCH: Forall2 match_event tr_tgt tr_src) *)
         (STEP: Star L1 st_tgt0 tr_tgt st_tgt1)
@@ -1272,7 +1281,7 @@ Section SIM.
       exists (Tr.app thd Tr.ub). esplits; ss.
       - clear - STAR STUCK.
         eapply beh_of_state_star; et. unfold NoStuck in *.
-        repeat (Psimpl; des; unfold NW in *). clears st_src0. clear st_src0.
+        repeat (Psimpl; des; unfold NW in * ). clears st_src0. clear st_src0.
         pfold. econsr; ss; et. ii. exploit wf_angelic; ss; et. i; subst. exfalso.
         exploit STUCK0; ss; et.
       - r in B. des. subst. clear - MB.
@@ -1284,7 +1293,7 @@ Section SIM.
         eapply match_event_iff in Heq.
         eapply match_beh_cons; ss; et. rewrite <- behavior_app_assoc. ss.
     }
-  Qed.
+  Qed. *)
 
 End SIM.
 Hint Constructors _sim.
